Renamed compiler functions

javascript/jsComputeLib.sml
@@ -2,8 +2,8 @@ structure jsComputeLib = struct
 open preamble javascriptBackendTheory prettyPrintTheory
 
 	val add_ata_compset = computeLib.extend_compset [computeLib.Defs [
-			ata_exp_def,
-			ata_dec_def,
+			compile_exp_def,
+			compile_dec_def,
 			exp_toString_def
 		]]
 	val jseval = computeLib.compset_conv computeLib.the_compset [computeLib.Extenders [add_ata_compset]]
